raft-proofs/EndToEndLinearizability.v
@@ -333,7 +333,7 @@ Hint Extern 4 (@log_all_entries_interface _ _ _) => apply laei : typeclass_insta
 Hint Extern 4 (@append_entries_reply_sublog_interface _ _ _) => apply aersi : typeclass_instances.
 Hint Extern 4 (@log_properties_hold_on_leader_logs_interface _ _ _) => apply lpholli : typeclass_instances.
 Hint Extern 4 (@append_entries_request_reply_correspondence_interface _ _ _) => apply aerrci : typeclass_instances.
-Hint Extern 4 (@append_entries_leaders_interface _ _ _) => apply appendeli : typeclass_instances.
+Hint Extern 4 (@append_entries_leader_interface _ _ _) => apply appendeli : typeclass_instances.
 
 Section EndToEndProof.
   Context {orig_base_params : BaseParams}.
